src/CFG/CFG_Prune.thy
@@ -21,15 +21,18 @@ text \<open>
 subsection \<open>Interprocedural reachability\<close>
 
 (* One dependency step: u's abstract value feeds w's right-hand side, either
-   via an edge (u -> w) or a combine (call site or callee exit of w). *)
+   via an edge (u -> w) or a combine predecessor relation. *)
+definition cfg_succ_rel :: "cfg \<Rightarrow> (pp \<times> pp) set" where
+  "cfg_succ_rel g =
+     {(u, w). \<exists>a. (u, a, w) \<in> edges g} \<union>
+     {(u, w). \<exists>ct \<in> combines g. combine_call_node ct = u \<and> combine_return_node ct = w} \<union>
+     {(u, w). \<exists>ct \<in> combines g. combine_exit_node ct = u \<and> combine_return_node ct = w}"
+
 definition cfg_succ :: "cfg \<Rightarrow> pp \<Rightarrow> pp \<Rightarrow> bool" where
-  "cfg_succ g u w \<longleftrightarrow>
-     (\<exists>a. (u, a, w) \<in> edges g)
-   \<or> (\<exists>e. (u, e, w) \<in> combines g)
-   \<or> (\<exists>c. (c, u, w) \<in> combines g)"
+  "cfg_succ g u w \<longleftrightarrow> (u, w) \<in> cfg_succ_rel g"
 
 definition cfg_reaches :: "cfg \<Rightarrow> pp \<Rightarrow> pp \<Rightarrow> bool" where
-  "cfg_reaches g v v0 \<longleftrightarrow> (v, v0) \<in> {(u, w). cfg_succ g u w}\<^sup>*"
+  "cfg_reaches g v v0 \<longleftrightarrow> (v, v0) \<in> (cfg_succ_rel g)^*"
 
 definition cone :: "cfg \<Rightarrow> pp \<Rightarrow> pp set" where
   "cone g v0 = {v. cfg_reaches g v v0}"
@@ -38,7 +41,7 @@ definition prune_to :: "cfg \<Rightarrow> pp \<Rightarrow> cfg" where
   "prune_to g v0 =
      mk_cfg (cfg_entry g) (cfg_exit g)
        {e \<in> edges g. snd (snd e) \<in> cone g v0}
-       {ct \<in> combines g. snd (snd ct) \<in> cone g v0}"
+       {ct \<in> combines g. combine_return_node ct \<in> cone g v0}"
 
 definition prune_cfg :: "cfg \<Rightarrow> cfg" where
   "prune_cfg g = prune_to g (cfg_exit g)"
@@ -50,21 +53,20 @@ lemma cfg_reaches_refl: "cfg_reaches g v v"
 
 lemma cfg_succ_reaches:
   "cfg_succ g u w \<Longrightarrow> cfg_reaches g w v0 \<Longrightarrow> cfg_reaches g u v0"
-  by (auto simp: cfg_reaches_def intro: converse_rtrancl_into_rtrancl)
+  by (auto simp: cfg_succ_def cfg_reaches_def intro: converse_rtrancl_into_rtrancl)
 
 lemma cfg_succ_mono:
   assumes "edges g1 \<subseteq> edges g2" "combines g1 \<subseteq> combines g2" "cfg_succ g1 u w"
   shows "cfg_succ g2 u w"
-  using assms unfolding cfg_succ_def by blast
-
+  using assms unfolding cfg_succ_def cfg_succ_rel_def by blast
 lemma cfg_reaches_mono:
   assumes "edges g1 \<subseteq> edges g2" "combines g1 \<subseteq> combines g2" "cfg_reaches g1 v w"
   shows "cfg_reaches g2 v w"
 proof -
-  have "{(u, w). cfg_succ g1 u w} \<subseteq> {(u, w). cfg_succ g2 u w}"
-    using cfg_succ_mono[OF assms(1,2)] by auto
-  then have "{(u, w). cfg_succ g1 u w}\<^sup>* \<subseteq> {(u, w). cfg_succ g2 u w}\<^sup>*"
-    by (rule rtrancl_mono)
+  have sub: "cfg_succ_rel g1 \<subseteq> cfg_succ_rel g2"
+    using assms unfolding cfg_succ_rel_def by blast
+  have "(cfg_succ_rel g1)^* \<subseteq> (cfg_succ_rel g2)^*"
+    using sub by (rule rtrancl_mono)
   thus ?thesis using assms(3) unfolding cfg_reaches_def by blast
 qed
 
@@ -75,7 +77,7 @@ lemma edges_prune_to[simp]:
   by (simp add: prune_to_def)
 
 lemma combines_prune_to[simp]:
-  "combines (prune_to g v0) = {ct \<in> combines g. snd (snd ct) \<in> cone g v0}"
+  "combines (prune_to g v0) = {ct \<in> combines g. combine_return_node ct \<in> cone g v0}"
   by (simp add: prune_to_def)
 
 lemma cfg_entry_prune_to[simp]: "cfg_entry (prune_to g v0) = cfg_entry g"
@@ -96,36 +98,50 @@ lemma cfg_witness_prune_to:
   using assms
 proof (induction rule: cfg_witness.induct)
   case (entry v s Sa)
-  then show ?case
-    by (auto intro: cfg_witness.entry)
+  then show ?case by (auto intro: cfg_witness.entry)
 next
   case (edge u a v Sa s t)
   show ?case
   proof (rule impI)
     assume rv: "cfg_reaches g v v0"
+    have usucc: "cfg_succ g u v"
+      using edge.hyps(1) unfolding cfg_succ_def cfg_succ_rel_def by blast
     have ruv: "cfg_reaches g u v0"
-      using edge.hyps(1) rv cfg_succ_reaches unfolding cfg_succ_def by blast
-    have wu: "cfg_witness (prune_to g v0) Sa u s" using edge.IH ruv by blast
+      using cfg_succ_reaches[OF usucc rv] .
+    have wu: "cfg_witness (prune_to g v0) Sa u s"
+      using edge.IH ruv by blast
     have ev: "(u, a, v) \<in> edges (prune_to g v0)"
       using edge.hyps(1) rv by (simp add: cone_def)
     show "cfg_witness (prune_to g v0) Sa v t"
       by (rule cfg_witness.edge[OF ev wu edge.hyps(3)])
   qed
 next
-  case (combine c ex v Sa s t)
+  case (combine c ex v dst rex Sa sto t u)
   show ?case
   proof (rule impI)
     assume rv: "cfg_reaches g v v0"
+    have call_pred: "\<exists>ct\<in>combines g. combine_call_node ct = c \<and> combine_return_node ct = v"
+      using combine.hyps(1) by (intro bexI[of _ "(c, ex, v, dst, rex)"]) (auto simp: combine_call_node_def combine_return_node_def)
+    have csucc: "cfg_succ g c v"
+      unfolding cfg_succ_def cfg_succ_rel_def using call_pred by blast
+    have exit_pred: "\<exists>ct\<in>combines g. combine_exit_node ct = ex \<and> combine_return_node ct = v"
+      using combine.hyps(1) by (intro bexI[of _ "(c, ex, v, dst, rex)"]) (auto simp: combine_exit_node_def combine_return_node_def)
+    have exsucc: "cfg_succ g ex v"
+      unfolding cfg_succ_def cfg_succ_rel_def using exit_pred by blast
     have rc: "cfg_reaches g c v0"
-      using combine.hyps(1) rv cfg_succ_reaches unfolding cfg_succ_def by blast
-    have rex: "cfg_reaches g ex v0"
-      using combine.hyps(1) rv cfg_succ_reaches unfolding cfg_succ_def by blast
-    have wc: "cfg_witness (prune_to g v0) Sa c s" using combine.IH(1) rc by blast
-    have wex: "cfg_witness (prune_to g v0) Sa ex t" using combine.IH(2) rex by blast
-    have cv: "(c, ex, v) \<in> combines (prune_to g v0)"
-      using combine.hyps(1) rv by (simp add: cone_def)
-    show "cfg_witness (prune_to g v0) Sa v <s|t>"
-      by (rule cfg_witness.combine[OF cv wc wex])
+      using cfg_succ_reaches[OF csucc rv] .
+    have rex': "cfg_reaches g ex v0"
+      using cfg_succ_reaches[OF exsucc rv] .
+    have wc: "cfg_witness (prune_to g v0) Sa c sto"
+      using combine.IH(1) rc by blast
+    have wex: "cfg_witness (prune_to g v0) Sa ex t"
+      using combine.IH(2) rex' by blast
+    have rv': "cfg_reaches g (combine_return_node (c, ex, v, dst, rex)) v0"
+      using combine.hyps(1) rv by (simp add: combine_return_node_def)
+    have cv: "(c, ex, v, dst, rex) \<in> combines (prune_to g v0)"
+      using combine.hyps(1) rv' by (simp add: cone_def)
+    show "cfg_witness (prune_to g v0) Sa v u"
+      by (rule cfg_witness.combine[OF cv wc wex combine.hyps(4)])
   qed
 qed
 
@@ -152,15 +168,15 @@ lemma cfg_reaches_trans:
 
 lemma cfg_reaches_edge:
   "(u, a, w) \<in> edges g \<Longrightarrow> cfg_reaches g u w"
-  by (rule cfg_succ_imp_reaches) (auto simp: cfg_succ_def)
+  by (rule cfg_succ_imp_reaches) (auto simp: cfg_succ_def cfg_succ_rel_def)
 
 lemma cfg_reaches_combine_call:
-  "(u, e, w) \<in> combines g \<Longrightarrow> cfg_reaches g u w"
-  by (rule cfg_succ_imp_reaches) (auto simp: cfg_succ_def)
+  "ct \<in> combines g \<Longrightarrow> cfg_reaches g (combine_call_node ct) (combine_return_node ct)"
+  by (rule cfg_succ_imp_reaches) (auto simp: cfg_succ_def cfg_succ_rel_def)
 
 lemma cfg_reaches_combine_exit:
-  "(c, u, w) \<in> combines g \<Longrightarrow> cfg_reaches g u w"
-  by (rule cfg_succ_imp_reaches) (auto simp: cfg_succ_def)
+  "ct \<in> combines g \<Longrightarrow> cfg_reaches g (combine_exit_node ct) (combine_return_node ct)"
+  by (rule cfg_succ_imp_reaches) (auto simp: cfg_succ_def cfg_succ_rel_def)
 
 lemma cfg_reaches_mk_mono:
   assumes "E1 \<subseteq> E2" "C1 \<subseteq> C2"
@@ -180,85 +196,105 @@ next
 next
   case (Seq c1 c2)
   obtain n1 en1 ex1 E1 C1 n2 en2 ex2 E2 C2 where
-        c1: "compile \<Pi> lay c1 n = (n1, en1, ex1, E1, C1)"
-    and c2: "compile \<Pi> lay c2 n1 = (n2, en2, ex2, E2, C2)"
+      c1': "compile \<Pi> lay c1 n = (n1, en1, ex1, E1, C1)"
+    and c2': "compile \<Pi> lay c2 n1 = (n2, en2, ex2, E2, C2)"
     and res: "en = en1" "ex = ex2"
              "E = E1 \<union> (if ex1 = en2 then {} else {(ex1, EA_Nop, en2)}) \<union> E2" "C = C1 \<union> C2"
     using Seq.prems by (auto split: prod.splits)
   have r1: "cfg_reaches (mk_cfg en ex E C) en1 ex1"
-  proof (rule cfg_reaches_mk_mono)
-    show "E1 \<subseteq> E" using res by auto
-    show "C1 \<subseteq> C" using res by auto
-    show "cfg_reaches (mk_cfg en1 ex1 E1 C1) en1 ex1" using Seq.IH(1)[OF c1] .
-  qed
+    by (rule cfg_reaches_mk_mono[OF _ _ Seq.IH(1)[OF c1']]) (use res in auto)
   have r2: "cfg_reaches (mk_cfg en ex E C) en2 ex2"
-  proof (rule cfg_reaches_mk_mono)
-    show "E2 \<subseteq> E" using res by auto
-    show "C2 \<subseteq> C" using res by auto
-    show "cfg_reaches (mk_cfg en2 ex2 E2 C2) en2 ex2" using Seq.IH(2)[OF c2] .
-  qed
+    by (rule cfg_reaches_mk_mono[OF _ _ Seq.IH(2)[OF c2']]) (use res in auto)
   have re: "cfg_reaches (mk_cfg en ex E C) ex1 en2"
     using res by (auto intro: cfg_reaches_edge cfg_reaches_refl)
-  show ?case
-    using r1 re r2 res cfg_reaches_trans by blast 
+  show ?case using r1 r2 re res cfg_reaches_trans by blast
 next
   case (If b c1 c2)
   obtain n1 en1 ex1 E1 C1 n2 en2 ex2 E2 C2 where
-        c1: "compile \<Pi> lay c1 (Suc n) = (n1, en1, ex1, E1, C1)"
-    and c2: "compile \<Pi> lay c2 n1 = (n2, en2, ex2, E2, C2)"
+      c1': "compile \<Pi> lay c1 (Suc n) = (n1, en1, ex1, E1, C1)"
+    and c2': "compile \<Pi> lay c2 n1 = (n2, en2, ex2, E2, C2)"
     and res: "en = n" "ex = n2"
-             "E = {(n, EA_Assume b, en1), (n, EA_AssumeNot b, en2)} \<union> E1 \<union> E2
-                   \<union> {(ex1, EA_Nop, n2), (ex2, EA_Nop, n2)}"
+             "E = {(n, EA_Assume b, en1), (n, EA_AssumeNot b, en2)} \<union> E1 \<union> E2 \<union> {(ex1, EA_Nop, n2), (ex2, EA_Nop, n2)}"
              "C = C1 \<union> C2"
     using If.prems by (auto split: prod.splits)
   have e_en1: "cfg_reaches (mk_cfg en ex E C) n en1"
     using res by (auto intro: cfg_reaches_edge)
   have r1: "cfg_reaches (mk_cfg en ex E C) en1 ex1"
-  proof (rule cfg_reaches_mk_mono)
-    show "E1 \<subseteq> E" using res by auto
-    show "C1 \<subseteq> C" using res by auto
-    show "cfg_reaches (mk_cfg en1 ex1 E1 C1) en1 ex1" using If.IH(1)[OF c1] .
-  qed
+    by (rule cfg_reaches_mk_mono[OF _ _ If.IH(1)[OF c1']]) (use res in auto)
   have ex1_xn: "cfg_reaches (mk_cfg en ex E C) ex1 n2"
     using res by (auto intro: cfg_reaches_edge)
-  show ?case
-    using e_en1 r1 ex1_xn res by (auto intro: cfg_reaches_trans)
+  show ?case using e_en1 r1 ex1_xn res cfg_reaches_trans by blast
 next
   case (While b c)
   obtain n1 en1 ex1 E1 C1 where
-        cc: "compile \<Pi> lay c (Suc n) = (n1, en1, ex1, E1, C1)"
+      cc: "compile \<Pi> lay c (Suc n) = (n1, en1, ex1, E1, C1)"
     and res: "en = n" "ex = n1"
-             "E = {(n, EA_Assume b, en1), (n, EA_AssumeNot b, n1)} \<union> E1
-                   \<union> {(ex1, EA_Nop, n)}"
+             "E = {(n, EA_Assume b, en1), (n, EA_AssumeNot b, n1)} \<union> E1 \<union> {(ex1, EA_Nop, n)}"
              "C = C1"
     using While.prems by (auto split: prod.splits)
   show ?case using res by (auto intro: cfg_reaches_edge)
 next
   case (Scope c)
   obtain m ein exin Ein Cin where
-        cc: "compile \<Pi> lay c (Suc n) = (m, ein, exin, Ein, Cin)"
+      cc: "compile \<Pi> lay c (Suc n) = (m, ein, exin, Ein, Cin)"
     and res: "en = n" "ex = m"
-             "E = Ein \<union> {(n, EA_Enter, ein)}"
-             "C = Cin \<union> {(n, exin, m)}"
+             "E = Ein \<union> {(n, EA_Enter [] [], ein)}"
+             "C = Cin \<union> {(n, exin, m, None, None)}"
     using Scope.prems by (auto split: prod.splits)
-  show ?case using res by (auto intro: cfg_reaches_combine_call)
+  have comb: "(n, exin, m, None, None) \<in> C"
+    using res by auto
+  have comb_cfg: "(n, exin, m, None, None) \<in> combines (mk_cfg en ex E C)"
+    using comb res by simp
+  have r: "cfg_reaches (mk_cfg en ex E C) (combine_call_node (n, exin, m, None, None)) (combine_return_node (n, exin, m, None, None))"
+    using comb_cfg by (rule cfg_reaches_combine_call)
+  show ?case using r res by (simp add: combine_call_node_def combine_return_node_def)
 next
-  case (Call p)
+  case (Call dst p actuals)
   show ?case
-  proof (cases "lay p")
+  proof (cases "\<Pi> p")
     case None
-    then show ?thesis using Call.prems by (auto intro: cfg_reaches_refl)
+    then show ?thesis using Call.prems by (auto split: option.splits prod.splits intro: cfg_reaches_refl)
   next
-    case (Some info)
-    obtain en_p ex_p E_p C_p where info: "info = (en_p, ex_p, E_p, C_p)"
-      by (cases info)
-    have res: "en = n" "ex = n + 1" "E = {(n, EA_Enter, en_p)}" "C = {(n, ex_p, n + 1)}"
-      using Call.prems Some info by auto
-    show ?thesis using res by (auto intro: cfg_reaches_combine_call)
+    case (Some decl)
+    have PIp[simp]: "\<Pi> p = Some decl"
+      using Some by simp
+    show ?thesis
+    proof (cases "lay p")
+      case None
+      then show ?thesis using Call.prems Some by (auto split: prod.splits intro: cfg_reaches_refl)
+    next
+      case (Some info)
+      then obtain en_p ex_p Ns_p E_p C_p where info'[simp]: "info = (en_p, ex_p, Ns_p, E_p, C_p)"
+        by (cases info) simp
+      have layp[simp]: "lay p = Some (en_p, ex_p, Ns_p, E_p, C_p)"
+        using Some by simp
+      have eq:
+        "(n + 2, n, n + 1,
+          {(n, EA_Enter (formals decl) actuals, en_p)},
+          {(n, ex_p, n + 1, dst, result decl)}) = (n', en, ex, E, C)"
+        using Call.prems by auto
+      have en_n[simp]: "en = n" and ex_n[simp]: "ex = n + 1"
+        using eq by simp_all
+      have E_n[simp]: "E = {(n, EA_Enter (formals decl) actuals, en_p)}"
+        and C_n[simp]: "C = {(n, ex_p, n + 1, dst, result decl)}"
+        using eq by simp_all
+      have comb: "(n, ex_p, n + 1, dst, result decl) \<in> C"
+        by simp
+      have comb_cfg: "(n, ex_p, n + 1, dst, result decl) \<in> combines (mk_cfg en ex E C)"
+        using comb by simp
+      have r: "cfg_reaches (mk_cfg en ex E C) (combine_call_node (n, ex_p, n + 1, dst, result decl)) (combine_return_node (n, ex_p, n + 1, dst, result decl))"
+        using comb_cfg by (rule cfg_reaches_combine_call)
+      have r': "cfg_reaches (mk_cfg en ex E C) n (n + 1)"
+        using r by (simp add: combine_call_node_def combine_return_node_def)
+      show ?thesis using r' by simp
+    qed
   qed
 next
-  case Restore
-  then show ?case by (auto intro: cfg_reaches_refl)
+  case (RestoreInternal r)
+  then have [simp]: "n' = n" "en = n" "ex = n" "E = {}" "C = {}"
+    by simp_all
+  show ?case
+    by (simp add: cfg_reaches_refl)
 qed
 
 lemma compile_prog_entry_cfg_reaches_exit:
